only todo left on examples are hello world and serialization

examples/contractMorphisms/optimizing/optimizing.v
@@ -20,13 +20,28 @@ Import ListNotations.
 Open Scope N_scope.
 Open Scope string.
 
+(** An example that shows how one might use a contract isomorphism to prove that an
+    optimized contract is behaviorally equivalent to its predecessor.
+
+    In this example, C has some extra, unnecessary data in storage. Since a large storage 
+    leads to gas inefficiency, one very simple optimization tactic might be to eliminate 
+    the extra data in storage. We do so, and prove an isomorphism.
+
+    This example also shows that isomorphisms are very strong, and in practice what is 
+    probably preferred would be a contract equivalence, or a bisimulation, which is 
+    weaker than an isomorphism but harder to prove.
+*)
+
+Section ContractOptimization.
 Context { Base : ChainBase }.
 Set Primitive Projections.
 Set Nonrecursive Elimination Schemes.
 
+Axiom todo : string -> forall {A}, A.
+
 Section Contract.
 Inductive entrypoint := | incr (u : unit).
-Record storage := build_storage { n_1 : N ; n_2 : N }.
+Record storage := build_storage { n_1 : N ; extra_data : unit }.
 Definition setup := N.
 Definition error := N.
 Definition result : Type := ResultMonad.result (storage * list ActionBody) error.
@@ -34,20 +49,19 @@ Definition result : Type := ResultMonad.result (storage * list ActionBody) error
 Section Serialization.
     Global Instance entrypoint_serializable : Serializable entrypoint := 
     Derive Serializable entrypoint_rect<incr>.
-
     Global Instance storage_serializable : Serializable storage := todo "".
 End Serialization.
 
 (* init function definition *)
 Definition init (_ : Chain) (_ : ContractCallContext) (n : setup) :
     ResultMonad.result storage error := 
-    Ok ({| n_1 := n ; n_2 := n |}).
+    Ok ({| n_1 := n ; extra_data := tt |}).
 
 (* receive function definition *)
 Definition receive (_ : Chain) (_ : ContractCallContext) (st : storage) 
     (msg : option entrypoint) : result :=
     match msg with 
-    | Some (incr _) => Ok ({| n_1 := st.(n_1) + 1 ; n_2 := st.(n_1) + 1 ; |}, [])
+    | Some (incr _) => Ok ({| n_1 := st.(n_1) + 1 ; extra_data := tt ; |}, [])
     | None => Err 0
     end.
 
@@ -90,6 +104,7 @@ Definition C' : Contract setup' entrypoint' storage' error' :=
 
 End Contract'.
 
+
 Section Isomorphism.
 
 (* a morphism C -> C' *)
@@ -99,26 +114,21 @@ Definition setup_morph : setup -> setup' := id.
 Definition state_morph (st : storage) : storage' := {| n := st.(n_1) |}.
 Definition error_morph : error -> error' := id.
 
-Lemma init_coherence : forall c ctx s, 
-    (init_result_transform state_morph error_morph) ((Blockchain.init C) c ctx s) = 
-    (Blockchain.init C') c ctx (setup_morph s).
-Proof. auto. Qed.
+Lemma init_coherence : init_coherence_prop C C' setup_morph state_morph error_morph.
+Proof. now unfold init_coherence_prop. Qed.
 
-Lemma recv_coherence : forall c ctx st op_msg, 
-    (recv_result_transform state_morph error_morph) ((Blockchain.receive C) c ctx st op_msg) = 
-    (Blockchain.receive C') c ctx (state_morph st) (option_map msg_morph op_msg).
+Lemma recv_coherence : recv_coherence_prop C C' msg_morph state_morph error_morph.
 Proof.
+    unfold recv_coherence_prop.
     intros.
     simpl.
-    unfold recv_result_transform, receive, receive'.
+    unfold result_functor, receive, receive'.
     destruct op_msg; auto.
-    destruct e. 
-    unfold state_morph.
-    auto.
+    now destruct e.
 Qed.
 
 Definition f : ContractMorphism C C' := 
-    simple_cm msg_morph setup_morph state_morph error_morph 
+    build_contract_morphism C C' setup_morph msg_morph state_morph error_morph 
         init_coherence recv_coherence.
 
 (* a morphism C' -> C *)
@@ -126,84 +136,40 @@ Definition msg_morph' (e : entrypoint') : entrypoint :=
     match e with | incr' _ => incr tt end.
 Definition setup_morph' : setup' -> setup := id.
 Definition state_morph' (st : storage') : storage := 
-        {| n_1 := st.(n) ; n_2 := st.(n) ; |}.
+        {| n_1 := st.(n) ; extra_data := tt ; |}.
 Definition error_morph' : error' -> error := id.
 
-Lemma init_coherence' : forall c ctx s, 
-    (init_result_transform state_morph' error_morph') ((Blockchain.init C') c ctx s) = 
-    (Blockchain.init C) c ctx (setup_morph' s).
-Proof. auto. Qed.
+Lemma init_coherence' : init_coherence_prop C' C setup_morph' state_morph' error_morph'.
+Proof. now unfold init_coherence_prop. Qed.
 
-Lemma recv_coherence' : forall c ctx st op_msg, 
-    (recv_result_transform state_morph' error_morph') ((Blockchain.receive C') c ctx st op_msg) = 
-    (Blockchain.receive C) c ctx (state_morph' st) (option_map msg_morph' op_msg).
+Lemma recv_coherence' : recv_coherence_prop C' C msg_morph' state_morph' error_morph'.
 Proof.
+    unfold recv_coherence_prop.
     intros.
     simpl.
-    unfold recv_result_transform, receive, receive'.
+    unfold result_functor, receive, receive'.
     destruct op_msg; auto.
-    destruct e. 
-    unfold state_morph'.
-    auto.
+    now destruct e.
 Qed.
 
 Definition g : ContractMorphism C' C := 
-    simple_cm msg_morph' setup_morph' state_morph' error_morph' 
+    build_contract_morphism C' C setup_morph' msg_morph' state_morph' error_morph' 
         init_coherence' recv_coherence'.
-
-
-(* a quick lemma *)
-Lemma st_entries_eq : 
-    forall bstate caddr cstate,
-    env_contracts bstate caddr = Some (C : WeakContract) ->
-    contract_state bstate caddr = Some cstate -> 
-    cstate.(n_1) = cstate.(n_2).
-Proof.
-Admitted.
 
 
 (* f and g are isomorphisms *)
 Theorem c_c'_equivalent : is_iso_cm f g.
 Proof.
-    unfold is_iso_cm.
-    split.
-    -   unfold composition_cm, id_cm.
-        apply is_eq_cm.
-        +   apply is_eq_cm_init.
-            *   apply functional_extensionality.
-                intro x. destruct x as [(c, ctx) s].
-                simpl.
-                unfold setup_morph, setup_morph', id_fun.
-                auto.
-            *   apply functional_extensionality.
-                intro x. destruct x; auto.
-                simpl.
-                unfold setup_morph, setup_morph', id_fun.
-                unfold state_morph, state_morph'.
-                destruct t.
-                simpl.
-                admit.
-                (* state morph is not an iso/you  *)
-        +   apply is_eq_cm_recv.
-            *   apply functional_extensionality.
-                intro x. destruct x as [((c, ctx), st) msg].
-                simpl.
-                unfold state_morph, state_morph', msg_morph, msg_morph', id_fun.
-                destruct msg.
-                **  destruct e. cbn.
-                    destruct st. cbn.
-                    destruct u.
-                    admit. (* same issue *)
-                **  destruct st. cbn.
-                    admit. (* same issue *)  
-            *   apply functional_extensionality.
-                intro x. destruct x; auto.
-                destruct t as [st acts].
-                simpl.
-                unfold state_morph, state_morph', id_fun.
-                destruct st. 
-                simpl.
-                admit. (* same issue *)
-Admitted.
+    unfold is_iso_cm, compose_cm, id_cm.
+    split; apply eq_cm; cbn;
+    unfold setup_morph, setup_morph', msg_morph, msg_morph', state_morph, state_morph',
+        error_morph, error_morph';
+    auto;
+    apply functional_extensionality;
+    intros.
+    -   now destruct x, u.
+    -   now destruct x, extra_data0.
+    -   now destruct x, u.
+Qed.
 
 End Isomorphism.
